<?xml version="1.0"?>
<rdf:RDF xmlns="https://w3id.org/isoiec5087/-1/v1/"
     xml:base="https://w3id.org/isoiec5087/-1/v1/"
     xmlns:cc="http://creativecommons.org/ns#"
     xmlns:dcterms="http://purl.org/dc/terms/"
     xmlns:owl="http://www.w3.org/2002/07/owl#"
     xmlns:rdf="http://www.w3.org/1999/02/22-rdf-syntax-ns#"
     xmlns:rdfs="http://www.w3.org/2000/01/rdf-schema#"
     xmlns:skos="http://www.w3.org/2004/02/skos/core#"
     xmlns:vann="http://purl.org/vocab/vann/"
     xmlns:xml="http://www.w3.org/XML/1998/namespace"
     xmlns:xsd="http://www.w3.org/2001/XMLSchema#"
     xmlns:i72="https://w3id.org/isoiec21972/v1/"
     xmlns:prov="http://www.w3.org/ns/prov#"
     xmlns:org="http://www.w3.org/ns/org#"
     xmlns:time="http://www.w3.org/2006/time#">
    <owl:Ontology rdf:about="https://w3id.org/isoiec5087/-1/v1/">
    	<!-- Identity -->
    	<dcterms:title>Information technology - City data model - Part 1: Foundation level concepts</dcterms:title>
        <rdfs:seeAlso rdf:resource="https://www.iso.org/standard/80718.html"/>
        <dcterms:bibliographicCitation>ISO/IEC 5087-1:2023</dcterms:bibliographicCitation>
    	<skos:definition>This ontology specifies the foundation-level concepts of the city data model.</skos:definition>
    	<vann:preferredNamespaceUri>https://w3id.org/isoiec5087/-1/v1/</vann:preferredNamespaceUri>
    	<vann:preferredNamespacePrefix>cdm1</vann:preferredNamespacePrefix>
    		
    	<!-- Provenance -->
        <dcterms:creator>Megan Katsumi</dcterms:creator>
        <dcterms:creator>Mark Fox</dcterms:creator>
    	<dcterms:creator>Kenneth Vaughn</dcterms:creator>
        <dcterms:issued rdf:datatype="http://www.w3.org/2001/XMLSchema#date">2023</dcterms:issued> <!-- Date of the source document, comment out if draft -->
        <owl:priorVersion rdf:datatype="http://www.w3.org/2001/XMLSchema#date">2017-11-05</owl:priorVersion> <!-- Date of prior ontology file, if any -->
		<dcterms:modified rdf:datatype="http://www.w3.org/2001/XMLSchema#date">2026-01-13</dcterms:modified> <!-- Date of this ontology file -->
        <owl:versionInfo>1.3.0</owl:versionInfo>
        <owl:versionIRI rdf:resource="https://w3id.org/isoiec5087/-1/v1/r3.0"/>
        <rdfs:comment>The prior version of this ontology was divided into a distinct file 
            for each pattern contained within Part 1; this version combines all of the 
            patterns into a single file for ease of reference. Some of the prior component 
            ontology files were labelled as v1.2. This update does not make any semantic
            changes from the approved ontology, but does correct several references 
            resulting in a change greater than a patch but less than a major change. As 
            such, it is published as v1.3.0.</rdfs:comment>
        
        <!-- License -->
        <cc:license>http://creativecommons.org/licenses/by/4.0/</cc:license>
        
        <!-- Imports -->
        <owl:imports rdf:resource="http://www.w3.org/ns/prov"/>
        <owl:imports rdf:resource="http://www.w3.org/ns/org"/>
        <owl:imports rdf:resource="http://www.w3.org/2006/time"/>
        <owl:imports rdf:resource="https://w3id.org/isoiec21972/v1"/>
    </owl:Ontology>
    

    <!-- 
    ///////////////////////////////////////////////////////////////////////////////////////
    //
    // Object Properties
    //
    ///////////////////////////////////////////////////////////////////////////////////////
     -->
    <!-- https://w3id.org/isoiec5087/-1/v1/CdmObjectProperty -->

    <owl:ObjectProperty rdf:about="https://w3id.org/isoiec5087/-1/v1/CdmObjectProperty">
        <skos:definition>Added for organizational purposes, to identify all object properties defined in the City Data Model.</skos:definition>
    </owl:ObjectProperty>


    <!-- https://w3id.org/isoiec5087/-1/v1/FoundationalCdmObjectProperty -->

    <owl:ObjectProperty rdf:about="https://w3id.org/isoiec5087/-1/v1/FoundationalCdmObjectProperty">
        <rdfs:subPropertyOf rdf:resource="https://w3id.org/isoiec5087/-1/v1/CdmObjectProperty"/>
        <skos:definition>Added for organizational purposes, to identify all foundational object properties defined in the City Data Model.</skos:definition>
    </owl:ObjectProperty>


    <!-- https://w3id.org/isoiec5087/-1/v1/CityUnitObjectProperty -->

    <owl:ObjectProperty rdf:about="https://w3id.org/isoiec5087/-1/v1/CityUnitObjectProperty">
        <rdfs:subPropertyOf rdf:resource="https://w3id.org/isoiec5087/-1/v1/FoundationalCdmObjectProperty"/>
        <skos:definition>Added for organizational purposes, to identify all city unit object properties defined in the City Data Model.</skos:definition>
    </owl:ObjectProperty>


    <!-- https://w3id.org/isoiec5087/-1/v1/LocationObjectProperty -->

    <owl:ObjectProperty rdf:about="https://w3id.org/isoiec5087/-1/v1/LocationObjectProperty">
        <rdfs:subPropertyOf rdf:resource="https://w3id.org/isoiec5087/-1/v1/FoundationalCdmObjectProperty"/>
        <skos:definition>Added for organizational purposes, to identify all location object properties defined in the City Data Model.</skos:definition>
    </owl:ObjectProperty>


    <!-- https://w3id.org/isoiec5087/-1/v1/MereologyObjectProperty -->

    <owl:ObjectProperty rdf:about="https://w3id.org/isoiec5087/-1/v1/MereologyObjectProperty">
        <rdfs:subPropertyOf rdf:resource="https://w3id.org/isoiec5087/-1/v1/FoundationalCdmObjectProperty"/>
        <skos:definition>Added for organizational purposes, to identify all mereology object properties defined in the City Data Model.</skos:definition>
    </owl:ObjectProperty>


    <!-- https://w3id.org/isoiec5087/-1/v1/RecurringEventObjectProperty -->

    <owl:ObjectProperty rdf:about="https://w3id.org/isoiec5087/-1/v1/RecurringEventObjectProperty">
        <rdfs:subPropertyOf rdf:resource="https://w3id.org/isoiec5087/-1/v1/FoundationalCdmObjectProperty"/>
        <skos:definition>Added for organizational purposes, to identify all recurring event object properties defined in the City Data Model.</skos:definition>
    </owl:ObjectProperty>


    <!-- https://w3id.org/isoiec5087/-1/v1/ResourceObjectProperty -->

    <owl:ObjectProperty rdf:about="https://w3id.org/isoiec5087/-1/v1/ResourceObjectProperty">
        <rdfs:subPropertyOf rdf:resource="https://w3id.org/isoiec5087/-1/v1/FoundationalCdmObjectProperty"/>
        <skos:definition>Added for organizational purposes, to identify all resource object properties defined in the City Data Model.</skos:definition>
    </owl:ObjectProperty>














        <!-- 
    ///////////////////////////////////////////////////////////////////////////////////////
    //
    // Object Properties
    //
    ///////////////////////////////////////////////////////////////////////////////////////
     -->





    <!-- 
    ///////////////////////////////////////////////////////////////////////////////////////
    //
    // Classes
    //
    ///////////////////////////////////////////////////////////////////////////////////////
     -->


    <!-- https://w3id.org/isoiec5087/-1/v1/CityUnitsThing -->

    <owl:Class rdf:about="https://w3id.org/isoiec5087/-1/v1/CityUnitsThing">
        <rdfs:comment>Added for organizational purposes to group the classes defined in the City Units portion of the CDM.</rdfs:comment>
        <rdfs:subClassOf rdf:resource="https://w3id.org/isoiec5087/-1/v1/FoundationalCdmThing"/>
    </owl:Class>
    




 
    <!-- 
    ///////////////////////////////////////////////////////////////////////////////////////
    //
    // Object Properties
    //
    ///////////////////////////////////////////////////////////////////////////////////////
     -->

    

    <!-- Issue: While aggregateOf is declared in ISO/IEC 5087-1, no definition is provided there or in the OWL files and it is never used in the document. It is also a generic term used in many other contexts (e.g., 5087-2). Thus, it is defined here generically without a range. -->
    <!-- https://w3id.org/isoiec5087/-1/v1/aggregateOf -->

    <owl:ObjectProperty rdf:about="https://w3id.org/isoiec5087/-1/v1/aggregateOf">
        <skos:definition>One object within a collection.</skos:definition>
        <rdfs:subPropertyOf rdf:resource="CityUnitObjectProperty"/>
    </owl:ObjectProperty>
    


    <!-- Issue: While aggregateOver is declared in ISO/IEC 5087-1, no definition is provided there or in the OWL files and it is never used in the document. The same concept seems to be called aggregationOf in ISO/IEC 5087-2, which is likely a more widely used term. Thus, aggregateOver is defined as a synonym to aggregationOf with a generic definition without a range. -->
    <!-- https://w3id.org/isoiec5087/-1/v1/aggregationOf -->

    <owl:ObjectProperty rdf:about="https://w3id.org/isoiec5087/-1/v1/aggregationOf">
        <skos:definition>A collection of objects.</skos:definition>
        <rdfs:subPropertyOf rdf:resource="LocationObjectProperty"/>
    </owl:ObjectProperty>
    
    <!-- https://w3id.org/isoiec5087/-1/v1/aggregateOver -->

    <owl:ObjectProperty rdf:about="https://w3id.org/isoiec5087/-1/v1/aggregateOver">
        <owl:equivalentProperty rdf:resource="https://w3id.org/isoiec5087/-1/v1/aggregationOf"/>
        <owl:deprecated rdf:datatype="http://www.w3.org/2001/XMLSchema#boolean">true</owl:deprecated>
        <rdfs:subPropertyOf rdf:resource="FoundationalCdmObjectProperty"/>
    </owl:ObjectProperty>
    
    <!-- Issue: ISO/IEC 5087-1 defines hasAggregateFunction with a range of "i72:function" but function is not defined in that document. This ontology defines a stub for Function with no real meaning. -->
    <!-- https://w3id.org/isoiec5087/-1/v1/hasAggregateFunction -->

    <owl:ObjectProperty rdf:about="https://w3id.org/isoiec5087/-1/v1/hasAggregateFunction">
        <rdfs:subPropertyOf rdf:resource="CityUnitObjectProperty"/>
        <rdfs:domain rdf:resource="https://w3id.org/isoiec21972/v1/Quantity"/>
        <rdfs:range rdf:resource="https://w3id.org/isoiec5087/-1/v1/Function"/>
    </owl:ObjectProperty>
    

    <!-- 
    ///////////////////////////////////////////////////////////////////////////////////////
    //
    // Data properties
    //
    ///////////////////////////////////////////////////////////////////////////////////////
     -->

    

    <!-- https://w3id.org/isoiec5087/-1/v1/hasRelativeYear -->

    <owl:DatatypeProperty rdf:about="https://w3id.org/isoiec5087/-1/v1/hasRelativeYear">
        <skos:definition>The base year used to define monetary values for a currency.</skos:definition>
        <rdfs:subPropertyOf rdf:resource="https://w3id.org/isoiec5087/-1/v1/CityUnitsDataProperty"/>
        <rdfs:range rdf:resource="http://www.w3.org/2001/XMLSchema#gYear"/>
    </owl:DatatypeProperty>
    

    <!-- 
    ///////////////////////////////////////////////////////////////////////////////////////
    //
    // Classes
    //
    ///////////////////////////////////////////////////////////////////////////////////////
     -->

    

    <!-- Issue: The class Acceleration is not defined in ISO/IEC 5087-1. -->
    <!-- https://w3id.org/isoiec5087/-1/v1/Acceleration -->

    <owl:Class rdf:about="https://w3id.org/isoiec5087/-1/v1/Acceleration">
        <rdfs:subClassOf rdf:resource="https://w3id.org/isoiec21972/v1/Quantity"/>
        <rdfs:subClassOf>
            <owl:Restriction>
                <owl:onProperty rdf:resource="https://w3id.org/isoiec21972/v1/value"/>
                <owl:allValuesFrom>
                    <owl:Restriction>
                        <owl:onProperty rdf:resource="https://w3id.org/isoiec21972/v1/unit_of_measure"/>
                        <owl:allValuesFrom rdf:resource="https://w3id.org/isoiec5087/-1/v1/AccelerationUnit"/>
                    </owl:Restriction>
                </owl:allValuesFrom>
            </owl:Restriction>
        </rdfs:subClassOf>
        <rdfs:label>acceleration</rdfs:label>
    </owl:Class>
    

    <!-- Issue: The class AccelerationUnit is not defined in ISO/IEC 5087-1 or i72. -->
    <!-- https://w3id.org/isoiec5087/-1/v1/AccelerationUnit -->

    <owl:Class rdf:about="https://w3id.org/isoiec5087/-1/v1/AccelerationUnit">
        <rdfs:subClassOf rdf:resource="https://w3id.org/isoiec21972/v1/Unit_of_measure"/>
        <rdfs:label>acceleration unit</rdfs:label>
    </owl:Class>
    

    <!-- Issue: The class AmountOfMoney is not defined in ISO/IEC 5087-1 or i72. -->
    <!-- https://w3id.org/isoiec5087/-1/v1/AmountOfMoney -->

    <owl:Class rdf:about="https://w3id.org/isoiec5087/-1/v1/AmountOfMoney">
        <rdfs:subClassOf rdf:resource="https://w3id.org/isoiec21972/v1/Quantity"/>
        <rdfs:subClassOf>
            <owl:Restriction>
                <owl:onProperty rdf:resource="https://w3id.org/isoiec21972/v1/value"/>
                <owl:allValuesFrom>
                    <owl:Restriction>
                        <owl:onProperty rdf:resource="https://w3id.org/isoiec21972/v1/unit_of_measure"/>
                        <owl:allValuesFrom rdf:resource="https://w3id.org/isoiec21972/v1/Monetary_unit"/>
                    </owl:Restriction>
                </owl:allValuesFrom>
            </owl:Restriction>
        </rdfs:subClassOf>
        <rdfs:label>amount of money</rdfs:label>
    </owl:Class>
    


    <!-- https://w3id.org/isoiec5087/-1/v1/Area -->

    <owl:Class rdf:about="https://w3id.org/isoiec5087/-1/v1/Area">
        <skos:definition>Area expresses the two-dimensional size of a defined part of a surface, typically a region bounded by a closed curve. It is a derived quantity in the International System of Units. Area is length squared.</skos:definition>
        <rdfs:label>area</rdfs:label>
        <rdfs:subClassOf rdf:resource="https://w3id.org/isoiec21972/v1/Quantity"/>
        <rdfs:subClassOf>
            <owl:Restriction>
                <owl:onProperty rdf:resource="https://w3id.org/isoiec21972/v1/value"/>
                <owl:allValuesFrom>
                    <owl:Restriction>
                        <owl:onProperty rdf:resource="https://w3id.org/isoiec21972/v1/unit_of_measure"/>
                        <owl:allValuesFrom rdf:resource="https://w3id.org/isoiec5087/-1/v1/AreaUnit"/>
                    </owl:Restriction>
                </owl:allValuesFrom>
            </owl:Restriction>
        </rdfs:subClassOf>
    </owl:Class>
    


    <!-- https://w3id.org/isoiec5087/-1/v1/AreaUnit -->

    <owl:Class rdf:about="https://w3id.org/isoiec5087/-1/v1/AreaUnit">
        <skos:definition>Unit of area in the specified system of units.</skos:definition>
        <rdfs:subClassOf rdf:resource="https://w3id.org/isoiec21972/v1/Unit_of_measure"/>
        <rdfs:label>area unit</rdfs:label>
    </owl:Class>
    

    <!-- Issue: The class Capacity is not defined in ISO/IEC 5087-1 or i72. -->
    <!-- https://w3id.org/isoiec5087/-1/v1/Capacity -->

    <owl:Class rdf:about="https://w3id.org/isoiec5087/-1/v1/Capacity">
        <rdfs:subClassOf rdf:resource="https://w3id.org/isoiec5087/-1/v1/CityUnitsThing"/>
        <rdfs:subClassOf>
            <owl:Restriction>
                <owl:onProperty rdf:resource="https://w3id.org/isoiec21972/v1/defined_by"/>
                <owl:minCardinality rdf:datatype="http://www.w3.org/2001/XMLSchema#nonNegativeInteger">1</owl:minCardinality>
            </owl:Restriction>
        </rdfs:subClassOf>
    </owl:Class>
    


    <!-- Issue: The class CapacityRate is not defined in ISO/IEC 5087-1 or i72. -->
    <!-- https://w3id.org/isoiec5087/-1/v1/CapacityRate -->

    <owl:Class rdf:about="https://w3id.org/isoiec5087/-1/v1/CapacityRate">
        <rdfs:subClassOf rdf:resource="https://w3id.org/isoiec21972/v1/Quantity"/>
        <rdfs:subClassOf>
            <owl:Restriction>
                <owl:onProperty rdf:resource="https://w3id.org/isoiec21972/v1/value"/>
                <owl:allValuesFrom>
                    <owl:Restriction>
                        <owl:onProperty rdf:resource="https://w3id.org/isoiec21972/v1/unit_of_measure"/>
                        <owl:allValuesFrom rdf:resource="https://w3id.org/isoiec5087/-1/v1/CardinalityUnitPerTime"/>
                    </owl:Restriction>
                </owl:allValuesFrom>
            </owl:Restriction>
        </rdfs:subClassOf>
        <!-- Issue: i72:cardinality_of is defined with a domain of Cardinality and a range of Population; it is applued -->
        <rdfs:subClassOf>
            <owl:Restriction>
                <owl:onProperty rdf:resource="https://w3id.org/isoiec21972/v1/cardinality_of"/>
                <owl:qualifiedCardinality rdf:datatype="http://www.w3.org/2001/XMLSchema#nonNegativeInteger">1</owl:qualifiedCardinality>
                <owl:onClass rdf:resource="https://w3id.org/isoiec5087/-1/v1/Capacity"/>
            </owl:Restriction>
        </rdfs:subClassOf>
    </owl:Class>
    


    <!-- Issue: The class CapacitySize is not defined in ISO/IEC 5087-1 or i72. -->
    <!-- https://w3id.org/isoiec5087/-1/v1/CapacitySize -->

    <owl:Class rdf:about="https://w3id.org/isoiec5087/-1/v1/CapacitySize">
        <rdfs:subClassOf rdf:resource="https://w3id.org/isoiec21972/v1/Quantity"/>
        <rdfs:subClassOf>
            <owl:Restriction>
                <owl:onProperty rdf:resource="https://w3id.org/isoiec21972/v1/value"/>
                <owl:allValuesFrom>
                    <owl:Restriction>
                        <owl:onProperty rdf:resource="https://w3id.org/isoiec21972/v1/unit_of_measure"/>
                        <owl:allValuesFrom rdf:resource="https://w3id.org/isoiec21972/v1/Cardinality_unit"/>
                    </owl:Restriction>
                </owl:allValuesFrom>
            </owl:Restriction>
        </rdfs:subClassOf>
        <rdfs:subClassOf>
            <owl:Restriction>
                <owl:onProperty rdf:resource="https://w3id.org/isoiec21972/v1/cardinality_of"/>
                <owl:qualifiedCardinality rdf:datatype="http://www.w3.org/2001/XMLSchema#nonNegativeInteger">1</owl:qualifiedCardinality>
                <owl:onClass rdf:resource="https://w3id.org/isoiec5087/-1/v1/Capacity"/>
            </owl:Restriction>
        </rdfs:subClassOf>
    </owl:Class>
    


    <!-- Issue: The class CardinalityMeasure is not defined in ISO/IEC 5087-1 or i72. -->
    <!-- https://w3id.org/isoiec5087/-1/v1/CardinalityMeasure -->

    <owl:Class rdf:about="https://w3id.org/isoiec5087/-1/v1/CardinalityMeasure">
        <rdfs:subClassOf rdf:resource="https://w3id.org/isoiec21972/v1/Measure"/>
        <rdfs:subClassOf>
            <owl:Restriction>
                <owl:onProperty rdf:resource="https://w3id.org/isoiec21972/v1/unit_of_measure"/>
                <owl:allValuesFrom rdf:resource="https://w3id.org/isoiec21972/v1/Cardinality_unit"/>
            </owl:Restriction>
        </rdfs:subClassOf>
    </owl:Class>
    


    <!-- Issue: The class CardinalityUnitPerTime is not defined in ISO/IEC 5087-1 or i72. -->
    <!-- https://w3id.org/isoiec5087/-1/v1/CardinalityUnitPerTime -->

    <owl:Class rdf:about="https://w3id.org/isoiec5087/-1/v1/CardinalityUnitPerTime">
        <rdfs:subClassOf rdf:resource="https://w3id.org/isoiec21972/v1/Unit_of_measureDivision"/>
        <rdfs:subClassOf>
            <owl:Restriction>
                <owl:onProperty rdf:resource="https://w3id.org/isoiec21972/v1/denominator"/>
                <owl:allValuesFrom rdf:resource="https://w3id.org/isoiec5087/-1/v1/TimeUnit"/>
            </owl:Restriction>
        </rdfs:subClassOf>
        <rdfs:subClassOf>
            <owl:Restriction>
                <owl:onProperty rdf:resource="https://w3id.org/isoiec21972/v1/numerator"/>
                <owl:allValuesFrom rdf:resource="https://w3id.org/isoiec21972/v1/Cardinality_unit"/>
            </owl:Restriction>
        </rdfs:subClassOf>
    </owl:Class>
    

    <!-- https://w3id.org/isoiec5087/-1/v1/Duration -->

    <owl:Class rdf:about="https://w3id.org/isoiec5087/-1/v1/Duration">
        <skos:definition>Duration is the amount of time that elapses between two instants or events.</skos:definition>
        <rdfs:label>duration</rdfs:label>
        <rdfs:subClassOf rdf:resource="https://w3id.org/isoiec21972/v1/Quantity"/>
        <rdfs:subClassOf rdf:resource="http://www.w3.org/2006/time#TemporalDuration"/>
        <rdfs:subClassOf>
            <owl:Restriction>
                <owl:onProperty rdf:resource="https://w3id.org/isoiec21972/v1/value"/>
                <owl:allValuesFrom>
                    <owl:Restriction>
                        <owl:onProperty rdf:resource="https://w3id.org/isoiec21972/v1/unit_of_measure"/>
                        <owl:allValuesFrom rdf:resource="https://w3id.org/isoiec5087/-1/v1/TimeUnit"/>
                    </owl:Restriction>
                </owl:allValuesFrom>
            </owl:Restriction>
        </rdfs:subClassOf>
    </owl:Class>
    


    <!-- Issue: ISO/IEC 5087-1 refers to the concept of "Function" and "function", but these are not defined in the document. This ontology defines a stub for Function with no real meaning. -->    <!-- https://w3id.org/isoiec5087/-1/v1/Function -->

    <owl:Class rdf:about="https://w3id.org/isoiec5087/-1/v1/Function">
        <rdfs:subClassOf rdf:resource="https://w3id.org/isoiec5087/-1/v1/CityUnitsThing"/>
        <rdfs:label>function</rdfs:label>
    </owl:Class>
    


    <!-- Issue: The class Geo_Position_unit is not defined in ISO/IEC 5087-1 or i72. -->
    <!-- https://w3id.org/isoiec5087/-1/v1/Geo_Position_unit -->

    <owl:Class rdf:about="https://w3id.org/isoiec5087/-1/v1/Geo_Position_unit">
        <rdfs:subClassOf rdf:resource="https://w3id.org/isoiec21972/v1/Unit_of_measure"/>
        <rdfs:comment>Reference systems to indicate geographic position.</rdfs:comment>
    </owl:Class>
    


    <!-- https://w3id.org/isoiec5087/-1/v1/Length -->

    <owl:Class rdf:about="https://w3id.org/isoiec5087/-1/v1/Length">
        <skos:definition>Length is the amount of space between two geographical points along a curve. It is a base quantity in the International System of Units and other systems of units. Length is speed times time. The metre, a base unit of length in the International System of Units, is defined in terms of speed of light during a certain time interval.</skos:definition>
        <rdfs:label>length</rdfs:label>
        <rdfs:subClassOf rdf:resource="https://w3id.org/isoiec21972/v1/Quantity"/>
        <rdfs:subClassOf>
            <owl:Restriction>
                <owl:onProperty rdf:resource="https://w3id.org/isoiec21972/v1/value"/>
                <owl:allValuesFrom>
                    <owl:Class>
                        <owl:intersectionOf rdf:parseType="Collection">
                            <rdf:Description rdf:about="https://w3id.org/isoiec21972/v1/Measure"/>
                            <owl:Restriction>
                                <owl:onProperty rdf:resource="https://w3id.org/isoiec21972/v1/unit_of_measure"/>
                                <owl:allValuesFrom rdf:resource="https://w3id.org/isoiec5087/-1/v1/LengthUnit"/>
                            </owl:Restriction>
                        </owl:intersectionOf>
                    </owl:Class>
                </owl:allValuesFrom>
            </owl:Restriction>
        </rdfs:subClassOf>
    </owl:Class>
    


    <!-- https://w3id.org/isoiec5087/-1/v1/LengthUnit -->

    <owl:Class rdf:about="https://w3id.org/isoiec5087/-1/v1/LengthUnit">
        <skos:definition>A specified system of units for distance.</skos:definition>
        <rdfs:subClassOf rdf:resource="https://w3id.org/isoiec21972/v1/Unit_of_measure"/>
        <rdfs:label>length unit</rdfs:label>
    </owl:Class>
    


    <!-- Issue: The class Mass is not defined in ISO/IEC 5087-1 or i72. -->
    <!-- https://w3id.org/isoiec5087/-1/v1/Mass -->

    <owl:Class rdf:about="https://w3id.org/isoiec5087/-1/v1/Mass">
        <rdfs:subClassOf rdf:resource="https://w3id.org/isoiec21972/v1/Quantity"/>
        <rdfs:subClassOf>
            <owl:Restriction>
                <owl:onProperty rdf:resource="https://w3id.org/isoiec21972/v1/value"/>
                <owl:allValuesFrom>
                    <owl:Restriction>
                        <owl:onProperty rdf:resource="https://w3id.org/isoiec21972/v1/unit_of_measure"/>
                        <owl:allValuesFrom rdf:resource="https://w3id.org/isoiec5087/-1/v1/MassUnit"/>
                    </owl:Restriction>
                </owl:allValuesFrom>
            </owl:Restriction>
        </rdfs:subClassOf>
        <rdfs:comment>Mass is the amount of matter of a phenomenon. It is a base quantity in the International System of Units. Mass is force divided by acceleration.</rdfs:comment>
        <rdfs:label>mass</rdfs:label>
    </owl:Class>
    


    <!-- Issue: The class MassUnit is not defined in ISO/IEC 5087-1 or i72. -->
    <!-- https://w3id.org/isoiec5087/-1/v1/MassUnit -->

    <owl:Class rdf:about="https://w3id.org/isoiec5087/-1/v1/MassUnit">
        <rdfs:subClassOf rdf:resource="https://w3id.org/isoiec21972/v1/Unit_of_measure"/>
        <rdfs:label>mass unit</rdfs:label>
    </owl:Class>
    


    <!-- https://w3id.org/isoiec5087/-1/v1/MonetaryValue -->

    <owl:Class rdf:about="https://w3id.org/isoiec5087/-1/v1/MonetaryValue">
        <skos:definition>A Monetary Value has a numerical value that is relative to a particular date (year). A Monetary Value is measured with some currency.</skos:definition>
        <rdfs:subClassOf rdf:resource="https://w3id.org/isoiec21972/v1/Measure"/>
        <rdfs:subClassOf>
            <owl:Restriction>
                <owl:onProperty rdf:resource="https://w3id.org/isoiec21972/v1/unit_of_measure"/>
                <owl:allValuesFrom rdf:resource="https://w3id.org/isoiec21972/v1/Monetary_unit"/>
            </owl:Restriction>
        </rdfs:subClassOf>
        <rdfs:subClassOf>
            <owl:Restriction>
                <owl:onProperty rdf:resource="https://w3id.org/isoiec5087/-1/v1/hasRelativeYear"/>
                <owl:qualifiedCardinality rdf:datatype="http://www.w3.org/2001/XMLSchema#nonNegativeInteger">1</owl:qualifiedCardinality>
                <owl:onDataRange rdf:resource="http://www.w3.org/2001/XMLSchema#gYear"/>
            </owl:Restriction>
        </rdfs:subClassOf>
    </owl:Class>
    


    <!-- https://w3id.org/isoiec5087/-1/v1/Ratio -->

    <owl:Class rdf:about="https://w3id.org/isoiec5087/-1/v1/Ratio">
        <skos:definition>A ratio is a comparison of two quantities, often expressed as a fraction or in the form a:b.</skos:definition>
        <rdfs:subClassOf rdf:resource="https://w3id.org/isoiec21972/v1/Quantity"/>
        <rdfs:label>ratio</rdfs:label>
    </owl:Class>
    


    <!-- https://w3id.org/isoiec5087/-1/v1/Speed -->

    <owl:Class rdf:about="https://w3id.org/isoiec5087/-1/v1/Speed">
        <skos:definition>Speed is the time rate of motion measured by the distance moved over in unit time.</skos:definition>
        <rdfs:label>speed</rdfs:label>
        <rdfs:subClassOf rdf:resource="https://w3id.org/isoiec21972/v1/Quantity"/>
        <rdfs:subClassOf>
            <owl:Restriction>
                <owl:onProperty rdf:resource="https://w3id.org/isoiec21972/v1/value"/>
                <owl:allValuesFrom>
                    <owl:Restriction>
                        <owl:onProperty rdf:resource="https://w3id.org/isoiec21972/v1/unit_of_measure"/>
                        <owl:allValuesFrom rdf:resource="https://w3id.org/isoiec5087/-1/v1/SpeedUnit"/>
                    </owl:Restriction>
                </owl:allValuesFrom>
            </owl:Restriction>
        </rdfs:subClassOf>
    </owl:Class>
    


    <!-- https://w3id.org/isoiec5087/-1/v1/SpeedUnit -->

    <owl:Class rdf:about="https://w3id.org/isoiec5087/-1/v1/SpeedUnit">
        <skos:definition>A specified system of units for speed.</skos:definition>
        <rdfs:subClassOf rdf:resource="https://w3id.org/isoiec21972/v1/Unit_of_measure"/>
        <rdfs:label>speed unit</rdfs:label>
    </owl:Class>
    


    <!-- https://w3id.org/isoiec5087/-1/v1/TimeUnit -->

    <owl:Class rdf:about="https://w3id.org/isoiec5087/-1/v1/TimeUnit">
        <skos:definition>A specified system of units for time.</skos:definition>
        <rdfs:subClassOf rdf:resource="https://w3id.org/isoiec21972/v1/Unit_of_measure"/>
        <rdfs:label>time unit</rdfs:label>
    </owl:Class>
    


    <!-- https://w3id.org/isoiec5087/-1/v1/ValueOfMoney -->

    <owl:Class rdf:about="https://w3id.org/isoiec5087/-1/v1/ValueOfMoney">
        <skos:definition>An amount of money that is defined relative to a particular year.</skos:definition>
        <rdfs:subClassOf rdf:resource="https://w3id.org/isoiec5087/-1/v1/AmountOfMoney"/>
        <rdfs:subClassOf>
            <owl:Restriction>
                <owl:onProperty rdf:resource="https://w3id.org/isoiec21972/v1/value"/>
                <owl:allValuesFrom rdf:resource="https://w3id.org/isoiec5087/-1/v1/MonetaryValue"/>
            </owl:Restriction>
        </rdfs:subClassOf>
    </owl:Class>
    


    <!-- https://w3id.org/isoiec5087/-1/v1/Volume -->

    <owl:Class rdf:about="https://w3id.org/isoiec5087/-1/v1/Volume">
        <skos:definition>Volume is a measure of how much three-dimensional space any phenomenon occupies. </skos:definition>
        <rdfs:label>volume</rdfs:label>
        <rdfs:subClassOf rdf:resource="https://w3id.org/isoiec21972/v1/Quantity"/>
        <rdfs:subClassOf>
            <owl:Restriction>
                <owl:onProperty rdf:resource="https://w3id.org/isoiec21972/v1/value"/>
                <owl:allValuesFrom>
                    <owl:Restriction>
                        <owl:onProperty rdf:resource="https://w3id.org/isoiec21972/v1/unit_of_measure"/>
                        <owl:allValuesFrom rdf:resource="https://w3id.org/isoiec5087/-1/v1/VolumeUnit"/>
                    </owl:Restriction>
                </owl:allValuesFrom>
            </owl:Restriction>
        </rdfs:subClassOf>
    </owl:Class>
    

    <!-- Issue: The class VolumeUnit is not defined in ISO/IEC 5087-1 or i72, but it is referenced in ISO/IEC 5087-1. -->
    <!-- https://w3id.org/isoiec5087/-1/v1/VolumeUnit -->

    <owl:Class rdf:about="https://w3id.org/isoiec5087/-1/v1/VolumeUnit">
        <skos:definition>A specified system of units for volume.</skos:definition>
        <rdfs:subClassOf rdf:resource="https://w3id.org/isoiec21972/v1/Unit_of_measure"/>
        <rdfs:label>volume unit</rdfs:label>
    </owl:Class>
    

    <!-- Issue: The classes Distinct_count is not defined in ISO/IEC 5087-1 or i72. -->
    <!-- https://w3id.org/isoiec21972/v1/Distinct_count -->

    <rdf:Description rdf:about="https://w3id.org/isoiec21972/v1/Distinct_count">
        <owl:equivalentClass rdf:resource="https://w3id.org/isoiec21972/v1/Population"/>
    </rdf:Description>
    

    <!-- Issue: The class System_of_units is not defined in ISO/IEC 5087-1 or i72 and is not referenced in this document. -->
    <!-- https://w3id.org/isoiec21972/v1/System_of_units -->

    <owl:Class rdf:about="https://w3id.org/isoiec21972/v1/System_of_units">
        <rdfs:subClassOf rdf:resource="https://w3id.org/isoiec5087/-1/v1/CityUnitsThing"/>
        <rdfs:comment>In order to achieve a coherent, interdependent set of units of measure in the wide variety of units that exist, units are organised in systems of units. A system of units is based on a set of units chosen by convention to be the system’s base units, units that are considered to be mutually independent (i.e., can’t be expressed in terms of each other).</rdfs:comment>
        <rdfs:label>system of units</rdfs:label>
    </owl:Class>
    


    <!-- Issue: The class Unit_of_measureDivision is not defined in ISO/IEC 5087-1 or i72. -->
    <!-- https://w3id.org/isoiec21972/v1/Unit_of_measureDivision -->

    <owl:Class rdf:about="https://w3id.org/isoiec21972/v1/Unit_of_measureDivision">
        <rdfs:subClassOf rdf:resource="https://w3id.org/isoiec21972/v1/Unit_of_measure"/>
        <rdfs:label>unit division</rdfs:label>
    </owl:Class>
    


    <!-- 
    ///////////////////////////////////////////////////////////////////////////////////////
    //
    // Individuals
    //
    ///////////////////////////////////////////////////////////////////////////////////////
     -->

    


    <!-- Issue: The class NAD83 is not defined in ISO/IEC 5087-1 or i72 and is not referenced in this document. -->
    <!-- https://w3id.org/isoiec5087/-1/v1/NAD83 -->

    <owl:NamedIndividual rdf:about="https://w3id.org/isoiec5087/-1/v1/NAD83">
        <rdf:type rdf:resource="https://w3id.org/isoiec5087/-1/v1/Geo_Position_unit"/>
        <rdfs:comment>North American Datum of 1983. A geodetic reference system.</rdfs:comment>
    </owl:NamedIndividual>
    


    <!-- Issue: The class WGS84 is not defined in ISO/IEC 5087-1 or i72 and is not referenced in this document. -->
    <!-- https://w3id.org/isoiec5087/-1/v1/WGS84 -->

    <owl:NamedIndividual rdf:about="https://w3id.org/isoiec5087/-1/v1/WGS84">
        <rdf:type rdf:resource="https://w3id.org/isoiec5087/-1/v1/Geo_Position_unit"/>
        <rdfs:comment>World Geodetic System of 1984. The reference system used by GPS.</rdfs:comment>
    </owl:NamedIndividual>
    

    <!-- Issue: ISO/IEC 5087-1 defines average with a rdf:type of "Function" but Function is never defined in the document. This ontology defines a stub for Function with no real meaning. -->
     <!-- Issue: ISO/IEC 5087-1 defines "average" as a class with the single property of rdf:type = Function, but there is no discussion of this concept in the text and it is unclear if the lower case "a" is a typo or if it is to indicate an individual rather than a class. Recommend deleting and adding in next minor version with necessary corrections. -->
    <!-- https://w3id.org/isoiec5087/-1/v1/average -->

    <owl:NamedIndividual rdf:about="https://w3id.org/isoiec5087/-1/v1/average">
        <rdf:type rdf:resource="https://w3id.org/isoiec5087/-1/v1/Function"/>
    </owl:NamedIndividual>

    <!-- 
    ///////////////////////////////////////////////////////////////////////////////////////
    //
    // Data properties
    //
    ///////////////////////////////////////////////////////////////////////////////////////
     -->

    <!-- https://w3id.org/isoiec5087/-1/v1/FoundationalCdmDataProperty -->

    <owl:DatatypeProperty rdf:about="https://w3id.org/isoiec5087/-1/v1/FoundationalCdmDataProperty">
        <skos:definition>Added for organizational purposes, to identify data properties defined in the Foundation-level CDM ontology.</skos:definition>
    </owl:DatatypeProperty>

    <!-- https://w3id.org/isoiec5087/-1/v1/CityUnitsDataProperty -->

    <owl:DatatypeProperty rdf:about="https://w3id.org/isoiec5087/-1/v1/CityUnitsDataProperty">
        <skos:definition>Added for organizational purposes, to identify data properties defined in the City Units Pattern of the CDM ontology.</skos:definition>
        <rdfs:subPropertyOf rdf:resource="https://w3id.org/isoiec5087/-1/v1/FoundationalCdmDataProperty"/>
    </owl:DatatypeProperty>


    <!-- https://w3id.org/isoiec5087/-1/v1/GeneralDataProperty -->

    <owl:DatatypeProperty rdf:about="https://w3id.org/isoiec5087/-1/v1/GeneralDataProperty">
        <skos:definition>Added for organizational purposes, to identify object properties defined in the General Properties Pattern of the CDM ontology.</skos:definition>
        <rdfs:subPropertyOf rdf:resource="https://w3id.org/isoiec5087/-1/v1/FoundationalCdmDataProperty"/>
    </owl:DatatypeProperty>


    <!-- https://w3id.org/isoiec5087/-1/v1/SpatialLocDataProperty -->

    <owl:DatatypeProperty rdf:about="https://w3id.org/isoiec5087/-1/v1/SpatialLocDataProperty">
        <skos:definition>Added for organizational purposes, to identify object properties defined in the Spatial Location Properties Pattern of the CDM ontology.</skos:definition>
        <rdfs:subPropertyOf rdf:resource="https://w3id.org/isoiec5087/-1/v1/FoundationalCdmDataProperty"/>
    </owl:DatatypeProperty>


    <!-- https://w3id.org/isoiec5087/-1/v1/RecurringEventDataProperty -->

    <owl:DatatypeProperty rdf:about="https://w3id.org/isoiec5087/-1/v1/RecurringEventDataProperty">
        <skos:definition>Added for organizational purposes, to identify object properties defined in the Recurring Event Properties Pattern of the CDM ontology.</skos:definition>
        <rdfs:subPropertyOf rdf:resource="https://w3id.org/isoiec5087/-1/v1/FoundationalCdmDataProperty"/>
    </owl:DatatypeProperty>



    <!-- https://w3id.org/isoiec5087/-1/v1/hasDescription -->

    <owl:DatatypeProperty rdf:about="https://w3id.org/isoiec5087/-1/v1/hasDescription">
        <skos:definition>Descriptive information about an object.</skos:definition>
        <rdfs:subPropertyOf rdf:resource="https://w3id.org/isoiec5087/-1/v1/GeneralDataProperty"/>
    </owl:DatatypeProperty>
    


    <!-- https://w3id.org/isoiec5087/-1/v1/hasIdentifier -->

    <owl:DatatypeProperty rdf:about="https://w3id.org/isoiec5087/-1/v1/hasIdentifier">
        <skos:definition>Unique identifier for an object.</skos:definition>
        <rdfs:subPropertyOf rdf:resource="https://w3id.org/isoiec5087/-1/v1/GeneralDataProperty"/>
    </owl:DatatypeProperty>
    


    <!-- https://w3id.org/isoiec5087/-1/v1/hasName -->

    <owl:DatatypeProperty rdf:about="https://w3id.org/isoiec5087/-1/v1/hasName">
        <skos:definition>Name of an object.</skos:definition>
        <rdfs:subPropertyOf rdf:resource="https://w3id.org/isoiec5087/-1/v1/GeneralDataProperty"/>
    </owl:DatatypeProperty>
    

    <!-- 
    ///////////////////////////////////////////////////////////////////////////////////////
    //
    // Object Properties
    //
    ///////////////////////////////////////////////////////////////////////////////////////
     -->

    <!-- Issue: ISO/IEC 5087-1 also defines "partOf" with a definition of "specifies a part-whole relationship between objects", but without any further definition (i.e., it has an empty row in the properties table and is not used as a parent class for any of the other properties.) It seems as if the intent was to define it and use it as a parent class for properPartOf -->

    <!-- Issue: It seems as if properPartOf, hasProperPart, componentOf, and hasComponent (and partOf, if defined) should be transitive properties. -->

    <!-- https://w3id.org/isoiec5087/-1/v1/componentOf -->

    <owl:ObjectProperty rdf:about="https://w3id.org/isoiec5087/-1/v1/componentOf">
        <rdfs:subPropertyOf rdf:resource="https://w3id.org/isoiec5087/-1/v1/properPartOf"/>
        <owl:inverseOf rdf:resource="https://w3id.org/isoiec5087/-1/v1/hasComponent"/>
        <skos:definition>Specifies a part-whole relationship between objects where the component is a part that is defined based on actual boundaries. The parts are often also defined according to distinct functions. For example, a headlight is a componentOf a car. </skos:definition>
    </owl:ObjectProperty>
    


    <!-- https://w3id.org/isoiec5087/-1/v1/hasComponent -->

    <owl:ObjectProperty rdf:about="https://w3id.org/isoiec5087/-1/v1/hasComponent">
        <skos:definition>Specifies a part-whole relationship between objects where the component is a part that is defined based on actual boundaries. The parts are often also defined according to distinct functions. For example, a car hasComponent headlight.</skos:definition>
        <rdfs:subPropertyOf rdf:resource="https://w3id.org/isoiec5087/-1/v1/hasProperPart"/>
    </owl:ObjectProperty>
    
  

    <!-- https://w3id.org/isoiec5087/-1/v1/hasProperPart -->

    <owl:ObjectProperty rdf:about="https://w3id.org/isoiec5087/-1/v1/hasProperPart">
        <skos:definition>Specifies a part-whole relationship between objects where an object cannot be part of itself.</skos:definition>
        <rdfs:subPropertyOf rdf:resource="https://w3id.org/isoiec5087/-1/v1/MereologyObjectProperty"/>
        <owl:inverseOf rdf:resource="https://w3id.org/isoiec5087/-1/v1/properPartOf"/>
    </owl:ObjectProperty>
    


    <!-- https://w3id.org/isoiec5087/-1/v1/immediateComponentOf -->

    <owl:ObjectProperty rdf:about="https://w3id.org/isoiec5087/-1/v1/immediateComponentOf">
        <skos:definition>Specifies a componentOf relationship where the if x immediateComponentOf y, then there does not exist a z where x immediateComponentOf z immediateComponentOf y.</skos:definition>
        <rdfs:subPropertyOf rdf:resource="https://w3id.org/isoiec5087/-1/v1/componentOf"/>
    </owl:ObjectProperty>
    


    <!-- https://w3id.org/isoiec5087/-1/v1/properPartOf -->

    <owl:ObjectProperty rdf:about="https://w3id.org/isoiec5087/-1/v1/properPartOf">
        <skos:definition>Specifies a part-whole relationship between objects where an object cannot be part of itself</skos:definition>
        <rdfs:subPropertyOf rdf:resource="https://w3id.org/isoiec5087/-1/v1/MereologyObjectProperty"/>
    </owl:ObjectProperty>
    


    <!-- 
    ///////////////////////////////////////////////////////////////////////////////////////
    //
    // Classes
    //
    ///////////////////////////////////////////////////////////////////////////////////////
     -->

    

    <!-- https://w3id.org/isoiec5087/-1/v1/Organization -->

    <owl:Class rdf:about="https://w3id.org/isoiec5087/-1/v1/Organization">
        <skos:definition>A collection of people organized together into a community or other social, commercial or political structure. The group has some common purpose or reason for existence which goes beyond the set of people belonging to it. An organization may itself be able to act as an agent.
        In addition to the standard http://www.w3.org/ns/org#Organization pattern, this ontology defines an Organization to be a subclass of an Agent.</skos:definition>
        <rdfs:subClassOf rdf:resource="https://w3id.org/isoiec5087/-1/v1/Agent"/>
        <rdfs:subClassOf rdf:resource="https://w3id.org/isoiec5087/-1/v1/OrganizationThing"/>
        <rdfs:subClassOf rdf:resource="http://www.w3.org/ns/org#Organization"/>
    </owl:Class>
    


    <!-- https://w3id.org/isoiec5087/-1/v1/OrganizationThing -->

    <owl:Class rdf:about="https://w3id.org/isoiec5087/-1/v1/OrganizationThing">
        <skos:definition>A class representing an organization in the context of the CDM ontology.</skos:definition>
        <rdfs:subClassOf rdf:resource="https://w3id.org/isoiec5087/-1/v1/FoundationalCdmThing"/>
    </owl:Class>
    

    <!-- Issue: There is nothing unique about the ISO/IEC 5087-1 Provenance Pattern and nothing under this class; recommend deleting. -->
    <!-- https://w3id.org/isoiec5087/-1/v1/ProvenanceThing -->

    <owl:Class rdf:about="https://w3id.org/isoiec5087/-1/v1/ProvenanceThing">
        <skos:definition>A class used to group classes within the provenance pattern.</skos:definition>
        <rdfs:subClassOf rdf:resource="https://w3id.org/isoiec5087/-1/v1/FoundationalCdmThing"/>
    </owl:Class>
    

    <!-- https://w3id.org/isoiec5087/-1/v1/AnnotationProperty -->

    <owl:AnnotationProperty rdf:about="https://w3id.org/isoiec5087/-1/v1/CdmAnnotationProperty"/>
    

    <!-- Issue: The class Literal is not defined in ISO/IEC 5087-1 or i72 and where it is used in this document seems to contain information inappropriate for an international standard. -->
    <!-- https://w3id.org/isoiec5087/-1/v1/Literal -->

    <owl:AnnotationProperty rdf:about="https://w3id.org/isoiec5087/-1/v1/Literal"/>
    

    <!-- 
    ///////////////////////////////////////////////////////////////////////////////////////
    //
    // Object Properties
    //
    ///////////////////////////////////////////////////////////////////////////////////////
    -->

    <!-- Issue: The property beginsRecurringState does not seem to have the correct definition in ISO/IEC 5087-1. As defined it is more of a pre-condition, while the term suggests a activation condition (i.e., it will occur as opposed to it may occur)-->
    <!-- https://w3id.org/isoiec5087/-1/v1/beginsRecurringState -->

    <owl:ObjectProperty rdf:about="https://w3id.org/isoiec5087/-1/v1/beginsRecurringState">
        <skos:definition>Defines a State that is required to be true in order to initiate the RecurringEvent.</skos:definition>
        <rdfs:subPropertyOf rdf:resource="https://w3id.org/isoiec5087/-1/v1/RecurringEventObjectProperty"/>
        <rdfs:domain rdf:resource="https://w3id.org/isoiec5087/-1/v1/RecurringEvent"/>
        <rdfs:range rdf:resource="https://w3id.org/isoiec5087/-1/v1/State"/>
    </owl:ObjectProperty>
    


    <!-- https://w3id.org/isoiec5087/-1/v1/beginsRecurringTime -->

    <owl:ObjectProperty rdf:about="https://w3id.org/isoiec5087/-1/v1/beginsRecurringTime">
        <skos:definition>Specifies the start time of the RecurringEvent’s activity with a time:TemporalEntity from the Time pattern.</skos:definition>
        <rdfs:subPropertyOf rdf:resource="https://w3id.org/isoiec5087/-1/v1/RecurringEventObjectProperty"/>
        <rdfs:domain rdf:resource="https://w3id.org/isoiec5087/-1/v1/RecurringEvent"/>
        <rdfs:range rdf:resource="http://www.w3.org/2006/time#TemporalEntity"/>
    </owl:ObjectProperty>
    

    <!-- Issue: The property endDayOfWeek is not defined in ISO/IEC 5087-1 or i72. -->
    <!-- https://w3id.org/isoiec5087/-1/v1/endDayOfWeek -->

    <owl:ObjectProperty rdf:about="https://w3id.org/isoiec5087/-1/v1/endDayOfWeek">
        <rdfs:subPropertyOf rdf:resource="https://w3id.org/isoiec5087/-1/v1/RecurringEventObjectProperty"/>
    </owl:ObjectProperty>
    

    <!-- Issue: The property endMonth is not defined in ISO/IEC 5087-1 or i72. -->
    <!-- https://w3id.org/isoiec5087/-1/v1/endMonth -->

    <owl:ObjectProperty rdf:about="https://w3id.org/isoiec5087/-1/v1/endMonth">
        <rdfs:subPropertyOf rdf:resource="https://w3id.org/isoiec5087/-1/v1/RecurringEventObjectProperty"/>
    </owl:ObjectProperty>
    


    <!-- Issue: The property endsRecurringState does not seem to have the correct definition in ISO/IEC 5087-1. As defined it is more of a pre-condition, while the term suggests a termination condition (i.e., it will occur as opposed to it may occur)-->
    <!-- https://w3id.org/isoiec5087/-1/v1/endsRecurringState -->

    <owl:ObjectProperty rdf:about="https://w3id.org/isoiec5087/-1/v1/endsRecurringState">
        <skos:definition>Defines a State that is required to be true in order terminate the RecurringEvent.</skos:definition>
        <rdfs:subPropertyOf rdf:resource="https://w3id.org/isoiec5087/-1/v1/RecurringEventObjectProperty"/>
        <rdfs:domain rdf:resource="https://w3id.org/isoiec5087/-1/v1/RecurringEvent"/>
        <rdfs:range rdf:resource="https://w3id.org/isoiec5087/-1/v1/State"/>
    </owl:ObjectProperty>
    


    <!-- https://w3id.org/isoiec5087/-1/v1/endsRecurringTime -->

    <owl:ObjectProperty rdf:about="https://w3id.org/isoiec5087/-1/v1/endsRecurringTime">
        <skos:definition>Specifies the end time of the RecurringEvent’s activity with a time:TemporalEntity from the Time pattern</skos:definition>
        <rdfs:subPropertyOf rdf:resource="https://w3id.org/isoiec5087/-1/v1/RecurringEventObjectProperty"/>
        <rdfs:domain rdf:resource="https://w3id.org/isoiec5087/-1/v1/RecurringEvent"/>
        <rdfs:range rdf:resource="http://www.w3.org/2006/time#TemporalEntity"/>
    </owl:ObjectProperty>
    

    
    <!-- https://w3id.org/isoiec5087/-1/v1/hasDayOfWeek -->

    <owl:ObjectProperty rdf:about="https://w3id.org/isoiec5087/-1/v1/hasDayOfWeek">
        <skos:definition>Specifies the day of the week on which a Weekly RecurringEvent occurs with the time:DayOfWeek class from the Time pattern.</skos:definition>
        <rdfs:subPropertyOf rdf:resource="https://w3id.org/isoiec5087/-1/v1/RecurringEventObjectProperty"/>
        <rdfs:domain rdf:resource="https://w3id.org/isoiec5087/-1/v1/WeeklyRecurringEvent"/>
        <!-- Issue: The class DayOfWeek is not defined in ISO/IEC 5087-1. -->
        <rdfs:range rdf:resource="http://www.w3.org/2006/time#DayOfWeek"/>
    </owl:ObjectProperty>
    

    <!-- Issue: The property hasMonth is not defined in ISO/IEC 5087-1 or i72 and is not used; although it is referenced in textual descriptions in this file but not in the standard. -->
    <!-- https://w3id.org/isoiec5087/-1/v1/hasMonth -->

    <owl:ObjectProperty rdf:about="https://w3id.org/isoiec5087/-1/v1/hasMonth">
        <rdfs:subPropertyOf rdf:resource="https://w3id.org/isoiec5087/-1/v1/RecurringEventObjectProperty"/>
    </owl:ObjectProperty>
    


    <!-- https://w3id.org/isoiec5087/-1/v1/hasOccurrence -->

    <owl:ObjectProperty rdf:about="https://w3id.org/isoiec5087/-1/v1/hasOccurrence">
        <skos:definition>Identifies the Activities that take place at the time and location.</skos:definition>
        <rdfs:subPropertyOf rdf:resource="https://w3id.org/isoiec5087/-1/v1/RecurringEventObjectProperty"/>
        <rdfs:domain rdf:resource="https://w3id.org/isoiec5087/-1/v1/RecurringEvent"/>
        <rdfs:range rdf:resource="https://w3id.org/isoiec5087/-1/v1/Activity"/>
    </owl:ObjectProperty>
    


    <!-- https://w3id.org/isoiec5087/-1/v1/hasSubRecurringEvent -->

    <owl:ObjectProperty rdf:about="https://w3id.org/isoiec5087/-1/v1/hasSubRecurringEvent">
        <skos:definition>identifies the sub-recurring events that comprise the RecurringEvent. As with an Activity, a RecurringEvent may be decomposed/decomposed into simpler/more complex RecurringEvents to support varying levels of granularity.</skos:definition>
        <rdfs:subPropertyOf rdf:resource="https://w3id.org/isoiec5087/-1/v1/RecurringEventObjectProperty"/>
        <rdfs:domain rdf:resource="https://w3id.org/isoiec5087/-1/v1/RecurringEvent"/>
        <rdfs:range rdf:resource="https://w3id.org/isoiec5087/-1/v1/RecurringEvent"/>
    </owl:ObjectProperty>
    


    <!-- https://w3id.org/isoiec5087/-1/v1/onDateTimeDescription -->

    <owl:ObjectProperty rdf:about="https://w3id.org/isoiec5087/-1/v1/onDateTimeDescription">
        <skos:definition>Specifies the date-time description (as defined in the Time pattern) on which a recurring event recurs. For example, the day of the month on which a MonthlyRecurringEvent recurs, or the day and month on which a YearlyRecurringEvent recurs.</skos:definition>
        <rdfs:subPropertyOf rdf:resource="https://w3id.org/isoiec5087/-1/v1/RecurringEventObjectProperty"/>
        <rdfs:domain rdf:resource="https://w3id.org/isoiec5087/-1/v1/RecurringEvent"/>
        <rdfs:range rdf:resource="http://www.w3.org/2006/time#DateTimeDescription"/>    
    </owl:ObjectProperty>
    

    <!-- https://w3id.org/isoiec5087/-1/v1/recursAddition -->

    <owl:ObjectProperty rdf:about="https://w3id.org/isoiec5087/-1/v1/recursAddition">
        <skos:definition>Defines a condition when the RecurringEvent should be added to. This can specify a time, day of the week, or specific dates.</skos:definition>
        <rdfs:subPropertyOf rdf:resource="https://w3id.org/isoiec5087/-1/v1/RecurringEventObjectProperty"/>
        <rdfs:domain rdf:resource="https://w3id.org/isoiec5087/-1/v1/RecurringEvent"/>
        <rdfs:range>
            <owl:Class>
                <owl:unionOf rdf:parseType="Collection">
                    <rdf:Description rdf:about="http://www.w3.org/2006/time#DayOfWeek"/>
                    <rdf:Description rdf:about="http://www.w3.org/2006/time#TemporalEntity"/>
                </owl:unionOf>
            </owl:Class>
        </rdfs:range>
    </owl:ObjectProperty>
    


    <!-- https://w3id.org/isoiec5087/-1/v1/recursExcept -->

    <owl:ObjectProperty rdf:about="https://w3id.org/isoiec5087/-1/v1/recursExcept">
        <skos:definition>Defines the exceptions for the RecurringEvent, i.e. conditions when it does not occur. This can specify a time, day of the week, or specific dates.</skos:definition>
        <rdfs:subPropertyOf rdf:resource="https://w3id.org/isoiec5087/-1/v1/RecurringEventObjectProperty"/>
        <rdfs:domain rdf:resource="https://w3id.org/isoiec5087/-1/v1/RecurringEvent"/>
        <rdfs:range>
            <owl:Class>
                <owl:unionOf rdf:parseType="Collection">
                    <rdf:Description rdf:about="http://www.w3.org/2006/time#DayOfWeek"/>
                    <rdf:Description rdf:about="http://www.w3.org/2006/time#TemporalEntity"/>
                </owl:unionOf>
            </owl:Class>
        </rdfs:range>
    </owl:ObjectProperty>
    


    <!-- https://w3id.org/isoiec5087/-1/v1/associatedLocation -->

    <owl:ObjectProperty rdf:about="https://w3id.org/isoiec5087/-1/v1/associatedLocation">
        <skos:definition>Captures the association of a non-spatial object with a Location. For example, an activity is not a spatial object but may be associated with some location in which it (mostly) takes place.</skos:definition>
        <rdfs:subPropertyOf rdf:resource="https://w3id.org/isoiec5087/-1/v1/LocationObjectProperty"/>
        <rdfs:range rdf:resource="https://w3id.org/isoiec5087/-1/v1/Location"/>
    </owl:ObjectProperty>
    


    <!-- 
    ///////////////////////////////////////////////////////////////////////////////////////
    //
    // Data properties
    //
    ///////////////////////////////////////////////////////////////////////////////////////
     -->


    <!-- https://w3id.org/isoiec5087/-1/v1/endTime -->

    <owl:DatatypeProperty rdf:about="https://w3id.org/isoiec5087/-1/v1/endTime">
        <skos:definition>Specifies the end time of the domain object's activity.</skos:definition>
        <rdfs:subPropertyOf rdf:resource="https://w3id.org/isoiec5087/-1/v1/RecurringEventDataProperty"/>
        <rdfs:domain rdf:resource="https://w3id.org/isoiec5087/-1/v1/RecurringEvent"/>
        <rdfs:range rdf:resource="http://www.w3.org/2001/XMLSchema#time"/>    
    </owl:DatatypeProperty>
    

    <!-- https://w3id.org/isoiec5087/-1/v1/startTime -->

    <owl:DatatypeProperty rdf:about="https://w3id.org/isoiec5087/-1/v1/startTime">
        <skos:definition>Specifies the start time of the RecurringEvent's activity using http://www.w3.org/2001/XMLSchema#time format.</skos:definition>
        <rdfs:subPropertyOf rdf:resource="https://w3id.org/isoiec5087/-1/v1/RecurringEventDataProperty"/>
        <rdfs:domain rdf:resource="https://w3id.org/isoiec5087/-1/v1/RecurringEvent"/>
        <rdfs:range rdf:resource="http://www.w3.org/2001/XMLSchema#time"/>    
    </owl:DatatypeProperty>
    


    <!-- 
    ///////////////////////////////////////////////////////////////////////////////////////
    //
    // Classes
    //
    ///////////////////////////////////////////////////////////////////////////////////////
     -->

    
    <!-- https://w3id.org/isoiec5087/-1/v1/DailyRecurringEvent -->

    <owl:Class rdf:about="https://w3id.org/isoiec5087/-1/v1/DailyRecurringEvent">
        <skos:definition>A DailyRecurringEvent is a RecurringEvent that occurs every day. It has a maximum of one associated time, the start time. Typically, a daily recurring event will occur at the same time every day, but it is also possible that no commitment is made to a recurring start time for the event, in which case no start time is specified. A DailyEvent does not necessarily have the same endtime or duration, therefore these are not specified.</skos:definition>
        <rdfs:subClassOf rdf:resource="https://w3id.org/isoiec5087/-1/v1/RecurringEvent"/>
        <rdfs:subClassOf>
            <owl:Restriction>
                <owl:onProperty rdf:resource="https://w3id.org/isoiec5087/-1/v1/startTime"/>
                <owl:maxQualifiedCardinality rdf:datatype="http://www.w3.org/2001/XMLSchema#nonNegativeInteger">1</owl:maxQualifiedCardinality>
                <owl:onDataRange rdf:resource="http://www.w3.org/2001/XMLSchema#time"/>
            </owl:Restriction>
        </rdfs:subClassOf>
    </owl:Class>
    

    <!-- Issue: ISO/IEC 5087-1 defines the range of onDateTimeDescription to be time:DateTimeDescription-->
    <!-- https://w3id.org/isoiec5087/-1/v1/ExceptionDay -->

    <owl:Class rdf:about="https://w3id.org/isoiec5087/-1/v1/ExceptionDay">
        <skos:definition>An ExceptionDay specifies a day or days that recursExcept and recursAddition use to specify unique days that do not recur on the same day each year, for example, holidays. </skos:definition>
        <rdfs:subClassOf rdf:resource="https://w3id.org/isoiec5087/-1/v1/RecurringEventThing"/>
        <rdfs:subClassOf>
            <owl:Restriction>
                <owl:onProperty rdf:resource="https://w3id.org/isoiec5087/-1/v1/onDateTimeDescription"/>
                <owl:someValuesFrom rdf:resource="http://www.w3.org/2006/time#GeneralDateTimeDescription"/>
            </owl:Restriction>
        </rdfs:subClassOf>
        <rdfs:subClassOf>
            <owl:Restriction>
                <owl:onProperty rdf:resource="https://w3id.org/isoiec5087/-1/v1/hasName"/>
                <owl:someValuesFrom rdf:resource="http://www.w3.org/2001/XMLSchema#string"/>
            </owl:Restriction>
        </rdfs:subClassOf>
    </owl:Class>
    


    <!-- Issue: ISO/IEC 5087-1 defines the range of onDateTimeDescription to be more restrictive -->
    <!-- https://w3id.org/isoiec5087/-1/v1/MonthlyRecurringEvent -->

    <owl:Class rdf:about="https://w3id.org/isoiec5087/-1/v1/MonthlyRecurringEvent">
        <skos:definition>A MonthlyRecurringEvent recurs regularly on the same day of each month, as specified by the dayOfMonth data property. Note that there is often ambiguity regarding the semantics of a monthly recurring event: in this formalization, a MonthlyRecurringEvent is any event that recurs regularly on the same day of each month; other interpretations sometimes consider events that recur on the same day of week, or first or last day, in which case the day of month will vary.</skos:definition>
        <rdfs:subClassOf rdf:resource="https://w3id.org/isoiec5087/-1/v1/RecurringEvent"/>
        <rdfs:subClassOf>
            <owl:Restriction>
                <owl:onProperty rdf:resource="https://w3id.org/isoiec5087/-1/v1/onDateTimeDescription"/>
                <owl:qualifiedCardinality rdf:datatype="http://www.w3.org/2001/XMLSchema#nonNegativeInteger">1</owl:qualifiedCardinality>
                <owl:onClass rdf:resource="http://www.w3.org/2006/time#GeneralDateTimeDescription"/>
            </owl:Restriction>
        </rdfs:subClassOf>
    </owl:Class>
    

    <!-- Issue: ISO/IEC 5087-1 includes a dayOfWeek property rather than a hasDayOfWeek property; according to the standard, the latter is limited to WeeklyRecurringEvent. It should likely be time:dayOfWeek.-->
    <!-- https://w3id.org/isoiec5087/-1/v1/RecurringEvent -->

    <owl:Class rdf:about="https://w3id.org/isoiec5087/-1/v1/RecurringEvent">
        <skos:definition>Recurring events are defined based on the regular interval at which they occur; this is captures using some combination of the hasTime, dayOfWeek, hasMonth, and dayOfMonth properties.  Using these properties, ontology defines the following specializations of the RecurringEvent class. Other subclasses may be defined similarly, as required.</skos:definition>
        <rdfs:subClassOf rdf:resource="https://w3id.org/isoiec5087/-1/v1/RecurringEventThing"/>
        <rdfs:subClassOf>
            <owl:Restriction>
                <owl:onProperty rdf:resource="https://w3id.org/isoiec5087/-1/v1/beginsRecurringState"/>
                <owl:allValuesFrom rdf:resource="https://w3id.org/isoiec5087/-1/v1/State"/>
            </owl:Restriction>
        </rdfs:subClassOf>
        <rdfs:subClassOf>
            <owl:Restriction>
                <owl:onProperty rdf:resource="https://w3id.org/isoiec5087/-1/v1/beginsRecurringTime"/>
                <owl:allValuesFrom rdf:resource="http://www.w3.org/2006/time#TemporalEntity"/>
            </owl:Restriction>
        </rdfs:subClassOf>
        <rdfs:subClassOf>
            <owl:Restriction>
                <owl:onProperty rdf:resource="https://w3id.org/isoiec5087/-1/v1/endsRecurringState"/>
                <owl:allValuesFrom rdf:resource="https://w3id.org/isoiec5087/-1/v1/State"/>
            </owl:Restriction>
        </rdfs:subClassOf>
        <rdfs:subClassOf>
            <owl:Restriction>
                <owl:onProperty rdf:resource="https://w3id.org/isoiec5087/-1/v1/endsRecurringTime"/>
                <owl:allValuesFrom rdf:resource="http://www.w3.org/2006/time#TemporalEntity"/>
            </owl:Restriction>
        </rdfs:subClassOf>
        <rdfs:subClassOf>
            <owl:Restriction>
                <owl:onProperty rdf:resource="https://w3id.org/isoiec5087/-1/v1/hasDayOfWeek"/>
                <owl:allValuesFrom rdf:resource="http://www.w3.org/2006/time#DayOfWeek"/>
            </owl:Restriction>
        </rdfs:subClassOf>
        <rdfs:subClassOf>
            <owl:Restriction>
                <owl:onProperty rdf:resource="https://w3id.org/isoiec5087/-1/v1/hasOccurrence"/>
                <owl:allValuesFrom rdf:resource="https://w3id.org/isoiec5087/-1/v1/Activity"/>
            </owl:Restriction>
        </rdfs:subClassOf>
        <rdfs:subClassOf>
            <owl:Restriction>
                <owl:onProperty rdf:resource="https://w3id.org/isoiec5087/-1/v1/hasSubRecurringEvent"/>
                <owl:allValuesFrom rdf:resource="https://w3id.org/isoiec5087/-1/v1/RecurringEvent"/>
            </owl:Restriction>
        </rdfs:subClassOf>
        <rdfs:subClassOf>
            <owl:Restriction>
                <owl:onProperty rdf:resource="https://w3id.org/isoiec5087/-1/v1/onDateTimeDescription"/>
                <owl:allValuesFrom rdf:resource="http://www.w3.org/2006/time#GeneralDateTimeDescription"/>
            </owl:Restriction>
        </rdfs:subClassOf>
        <rdfs:subClassOf>
            <owl:Restriction>
                <owl:onProperty rdf:resource="https://w3id.org/isoiec5087/-1/v1/recursAddition"/>
                <owl:allValuesFrom>
                    <owl:Class>
                        <owl:unionOf rdf:parseType="Collection">
                            <rdf:Description rdf:about="http://www.w3.org/2006/time#DayOfWeek"/>
                            <rdf:Description rdf:about="http://www.w3.org/2006/time#TemporalEntity"/>
                        </owl:unionOf>
                    </owl:Class>
                </owl:allValuesFrom>
            </owl:Restriction>
        </rdfs:subClassOf>
        <rdfs:subClassOf>
            <owl:Restriction>
                <owl:onProperty rdf:resource="https://w3id.org/isoiec5087/-1/v1/recursExcept"/>
                <owl:allValuesFrom>
                    <owl:Class>
                        <owl:unionOf rdf:parseType="Collection">
                            <rdf:Description rdf:about="http://www.w3.org/2006/time#DayOfWeek"/>
                            <rdf:Description rdf:about="http://www.w3.org/2006/time#TemporalEntity"/>
                        </owl:unionOf>
                    </owl:Class>
                </owl:allValuesFrom>
            </owl:Restriction>
        </rdfs:subClassOf>
        <rdfs:subClassOf>
            <owl:Restriction>
                <owl:onProperty rdf:resource="https://w3id.org/isoiec5087/-1/v1/associatedLocation"/>
                <owl:allValuesFrom rdf:resource="https://w3id.org/isoiec5087/-1/v1/Location"/>
            </owl:Restriction>
        </rdfs:subClassOf>
        <rdfs:subClassOf>
            <owl:Restriction>
                <owl:onProperty rdf:resource="https://w3id.org/isoiec5087/-1/v1/endTime"/>
                <owl:allValuesFrom rdf:resource="http://www.w3.org/2001/XMLSchema#time"/>
            </owl:Restriction>
        </rdfs:subClassOf>
        <rdfs:subClassOf>
            <owl:Restriction>
                <owl:onProperty rdf:resource="https://w3id.org/isoiec5087/-1/v1/startTime"/>
                <owl:allValuesFrom rdf:resource="http://www.w3.org/2001/XMLSchema#time"/>
            </owl:Restriction>
        </rdfs:subClassOf>
    </owl:Class>
    


    <!-- https://w3id.org/isoiec5087/-1/v1/RecurringEventThing -->

    <owl:Class rdf:about="https://w3id.org/isoiec5087/-1/v1/RecurringEventThing">
        <rdfs:comment>Class added for organizational purposes only; to group all classes defined in the recurring-event ontology.</rdfs:comment>
        <rdfs:subClassOf rdf:resource="https://w3id.org/isoiec5087/-1/v1/FoundationalCdmThing"/>
    </owl:Class>
    


    <!-- https://w3id.org/isoiec5087/-1/v1/WeeklyRecurringEvent -->

    <owl:Class rdf:about="https://w3id.org/isoiec5087/-1/v1/WeeklyRecurringEvent">
        <skos:definition>A WeeklyRecurringEvent recurs on the regularly on the same day of the week, as specified by the schema:dayOfWeek property.</skos:definition>
        <rdfs:subClassOf rdf:resource="https://w3id.org/isoiec5087/-1/v1/RecurringEvent"/>
        <rdfs:subClassOf>
            <owl:Restriction>
                <owl:onProperty rdf:resource="https://w3id.org/isoiec5087/-1/v1/hasDayOfWeek"/>
                <owl:qualifiedCardinality rdf:datatype="http://www.w3.org/2001/XMLSchema#nonNegativeInteger">1</owl:qualifiedCardinality>
                <owl:onClass rdf:resource="http://www.w3.org/2006/time#DayOfWeek"/>
            </owl:Restriction>
        </rdfs:subClassOf>
    </owl:Class>
    


    <!-- Issue: ISO/IEC 5087-1 defines the range of onDateTimeDescription to be more restrictive -->
    <!-- https://w3id.org/isoiec5087/-1/v1/YearlyRecurringEvent -->

    <owl:Class rdf:about="https://w3id.org/isoiec5087/-1/v1/YearlyRecurringEvent">
        <skos:definition>A YearlyRecurringEvent recurs regularly on the same day of the same month, as specified by the hasMonth and dayOfMonth properties. As with MonthlyRecurringEvent, there may be ambiguity regarding the semantics of a yearly recurring event, however this formalization captures only the notion of an event that recurs on the same day of the same month (e.g. a birthday).</skos:definition>
        <rdfs:subClassOf rdf:resource="https://w3id.org/isoiec5087/-1/v1/RecurringEvent"/>
        <rdfs:subClassOf>
            <owl:Restriction>
                <owl:onProperty rdf:resource="https://w3id.org/isoiec5087/-1/v1/onDateTimeDescription"/>
                <owl:qualifiedCardinality rdf:datatype="http://www.w3.org/2001/XMLSchema#nonNegativeInteger">1</owl:qualifiedCardinality>
                <owl:onClass rdf:resource="http://www.w3.org/2006/time#GeneralDateTimeDescription"/>
            </owl:Restriction>
        </rdfs:subClassOf>
    </owl:Class>
    


    <!-- https://w3id.org/isoiec5087/-1/v1/Location -->

    <owl:Class rdf:about="https://w3id.org/isoiec5087/-1/v1/Location">
        <skos:definition>A specialization (subclass) of geo:Geometry that refers to a geospatial representation of the space occupied by some object.</skos:definition>
        <rdfs:subClassOf rdf:resource="https://w3id.org/isoiec5087/-1/v1/FoundationalCdmThing"/>
        <rdfs:subClassOf rdf:resource="http://www.opengis.net/ont/geosparql#Geometry"/>
    </owl:Class>
    



    

    <!-- 
    ///////////////////////////////////////////////////////////////////////////////////////
    //
    // Object Properties
    //
    ///////////////////////////////////////////////////////////////////////////////////////
     -->

    


    <!-- https://w3id.org/isoiec5087/-1/v1/capacityInUse -->

    <owl:ObjectProperty rdf:about="https://w3id.org/isoiec5087/-1/v1/capacityInUse">
        <skos:definition>Identifies the portion of capacity in use, by some Activity(s).</skos:definition>
        <rdfs:subPropertyOf rdf:resource="https://w3id.org/isoiec5087/-1/v1/ResourceObjectProperty"/>
        <rdf:type rdf:resource="http://www.w3.org/2002/07/owl#FunctionalProperty"/>
        <rdfs:domain rdf:resource="https://w3id.org/isoiec5087/-1/v1/Resource"/>
        <rdfs:range rdf:resource="https://w3id.org/isoiec21972/v1/Quantity"/>    
    </owl:ObjectProperty>
    

    <!-- Issue: The property consumes is not defined in ISO/IEC 5087-1 -->
    <!-- https://w3id.org/isoiec5087/-1/v1/consumedBy -->

    <owl:ObjectProperty rdf:about="https://w3id.org/isoiec5087/-1/v1/consumedBy">
        <rdfs:subPropertyOf rdf:resource="https://w3id.org/isoiec5087/-1/v1/preconditionOf"/>
    </owl:ObjectProperty>
    


    <!-- https://w3id.org/isoiec5087/-1/v1/forResource -->

    <owl:ObjectProperty rdf:about="https://w3id.org/isoiec5087/-1/v1/forResource">
        <skos:definition>Specifies the Resource that is allocated.</skos:definition>
        <rdfs:subPropertyOf rdf:resource="https://w3id.org/isoiec5087/-1/v1/ResourceObjectProperty"/>
        <rdfs:domain rdf:resource="https://w3id.org/isoiec5087/-1/v1/PlannedAllocation"/>
        <rdfs:range rdf:resource="https://w3id.org/isoiec5087/-1/v1/Resource"/>    
    </owl:ObjectProperty>
    


    <!-- https://w3id.org/isoiec5087/-1/v1/forState -->

    <owl:ObjectProperty rdf:about="https://w3id.org/isoiec5087/-1/v1/forState">
        <skos:definition>Specifies the State to which the Resource is allocated.</skos:definition>
        <rdfs:subPropertyOf rdf:resource="https://w3id.org/isoiec5087/-1/v1/ResourceObjectProperty"/>
        <rdfs:domain rdf:resource="https://w3id.org/isoiec5087/-1/v1/PlannedAllocation"/>
        <rdfs:range rdf:resource="https://w3id.org/isoiec5087/-1/v1/State"/>  
        <owl:inverseOf rdf:resource="https://w3id.org/isoiec5087/-1/v1/hasAllocation"/>  
    </owl:ObjectProperty>
    


    <!-- https://w3id.org/isoiec5087/-1/v1/hasAllocation -->

    <owl:ObjectProperty rdf:about="https://w3id.org/isoiec5087/-1/v1/hasAllocation">
        <skos:definition>Specifies a Planned Allocation for the Resource. This indicates a State and time Interval to which the Resource has been allocated.</skos:definition>
        <rdfs:subPropertyOf rdf:resource="https://w3id.org/isoiec5087/-1/v1/ResourceObjectProperty"/>
    </owl:ObjectProperty>
    

    <!-- Issue: In ISO/IEC 5087-1, hasAsset is listed in a table as a null entry with no other reference and this file does not provide any additional information -->
    <!-- https://w3id.org/isoiec5087/-1/v1/hasAsset -->

    <owl:ObjectProperty rdf:about="https://w3id.org/isoiec5087/-1/v1/hasAsset">
        <rdfs:subPropertyOf rdf:resource="https://w3id.org/isoiec5087/-1/v1/ResourceObjectProperty"/>
    </owl:ObjectProperty>
    


    <!-- https://w3id.org/isoiec5087/-1/v1/hasAvailableCapacity -->

    <owl:ObjectProperty rdf:about="https://w3id.org/isoiec5087/-1/v1/hasAvailableCapacity">
        <skos:definition>identifies the Quantity that specifies how much of the Resource is available for use.</skos:definition>
        <rdfs:subPropertyOf rdf:resource="https://w3id.org/isoiec5087/-1/v1/ResourceObjectProperty"/>
        <rdfs:domain rdf:resource="https://w3id.org/isoiec5087/-1/v1/Resource"/>
        <rdfs:range rdf:resource="https://w3id.org/isoiec21972/v1/Quantity"/>    
    </owl:ObjectProperty>
    


    <!-- https://w3id.org/isoiec5087/-1/v1/hasCapacity -->

    <owl:ObjectProperty rdf:about="https://w3id.org/isoiec5087/-1/v1/hasCapacity">
        <skos:definition>Identifies the Quantity that specifies how much of the Resource exists, e.g. its volume, if it is liquid; how much it can hold, if it is an container.</skos:definition>
        <rdfs:subPropertyOf rdf:resource="https://w3id.org/isoiec5087/-1/v1/ResourceObjectProperty"/>
        <rdf:type rdf:resource="http://www.w3.org/2002/07/owl#FunctionalProperty"/>
        <rdfs:domain rdf:resource="https://w3id.org/isoiec5087/-1/v1/Resource"/>
        <rdfs:range rdf:resource="https://w3id.org/isoiec21972/v1/Quantity"/>    
    </owl:ObjectProperty>
    

    <!-- Issue: hasOwner is not defined in ISO/IEC 5087-1. -->
    <!-- https://w3id.org/isoiec5087/-1/v1/hasOwner -->

    <owl:ObjectProperty rdf:about="https://w3id.org/isoiec5087/-1/v1/hasOwner">
        <skos:definition>A Resource may have some owner. The owner of a resource is subject to change over time.</skos:definition>
        <rdfs:subPropertyOf rdf:resource="https://w3id.org/isoiec5087/-1/v1/ResourceObjectProperty"/>
        <owl:inverseOf rdf:resource="https://w3id.org/isoiec5087/-1/v1/ownedBy"/>
        <rdfs:domain rdf:resource="https://w3id.org/isoiec5087/-1/v1/Resource"/>
    </owl:ObjectProperty>
    

    <!-- https://w3id.org/isoiec5087/-1/v1/hasQuantity -->

    <owl:ObjectProperty rdf:about="https://w3id.org/isoiec5087/-1/v1/hasQuantity">
        <skos:definition>Specifies the Quantity of the Resource that participates in the State, if applicable.</skos:definition>
        <rdfs:subPropertyOf rdf:resource="https://w3id.org/isoiec5087/-1/v1/ResourceObjectProperty"/>
        <rdfs:domain rdf:resource="https://w3id.org/isoiec5087/-1/v1/PlannedAllocation"/>
        <rdfs:range rdf:resource="https://w3id.org/isoiec21972/v1/Quantity"/>    
    </owl:ObjectProperty>
    


    <!-- https://w3id.org/isoiec5087/-1/v1/hasResource -->

    <owl:ObjectProperty rdf:about="https://w3id.org/isoiec5087/-1/v1/hasResource">
        <skos:definition>Specifies a Resource that participates in the State. This identifies the condition of the object that plays a resource role (i.e. is used, consumed, etc.) when the state’s status is active.</skos:definition>
        <rdfs:subPropertyOf rdf:resource="https://w3id.org/isoiec5087/-1/v1/ResourceObjectProperty"/>
        <owl:inverseOf rdf:resource="https://w3id.org/isoiec5087/-1/v1/resourceOf"/>
        <rdfs:domain rdf:resource="https://w3id.org/isoiec5087/-1/v1/TerminalResourceState"/>
        <rdfs:range rdf:resource="https://w3id.org/isoiec5087/-1/v1/Resource"/>    
    </owl:ObjectProperty>
    

    <!-- Issue: ownedBy is not defined in ISO/IEC 5087-1. -->
    <!-- https://w3id.org/isoiec5087/-1/v1/ownedBy -->

    <owl:ObjectProperty rdf:about="https://w3id.org/isoiec5087/-1/v1/ownedBy">
        <rdfs:subPropertyOf rdf:resource="https://w3id.org/isoiec5087/-1/v1/ResourceObjectProperty"/>
    </owl:ObjectProperty>
    


    <!-- https://w3id.org/isoiec5087/-1/v1/participatesIn -->

    <owl:ObjectProperty rdf:about="https://w3id.org/isoiec5087/-1/v1/participatesIn">
        <skos:definition>Identifies the Activity that the Resource is being used, consumed, produced, or released by.</skos:definition>
        <rdfs:subPropertyOf rdf:resource="https://w3id.org/isoiec5087/-1/v1/ResourceObjectProperty"/>
        <rdfs:domain rdf:resource="https://w3id.org/isoiec5087/-1/v1/Resource"/>
        <rdfs:range rdf:resource="https://w3id.org/isoiec5087/-1/v1/Activity"/>    
    </owl:ObjectProperty>
    


    <!-- https://w3id.org/isoiec5087/-1/v1/resourceOf -->

    <owl:ObjectProperty rdf:about="https://w3id.org/isoiec5087/-1/v1/resourceOf">
        <skos:definition>identifies what State the agent may be a resource of. This is specified using the Resource pattern, where the Agent would be considered to be a resource from the perspective of an Activity that uses it in some way. For example, a construction activity may use some persons(s) and those persons would be considered a Resource for that Activity.</skos:definition>
        <rdfs:subPropertyOf rdf:resource="https://w3id.org/isoiec5087/-1/v1/ResourceObjectProperty"/>
    </owl:ObjectProperty>
    

    <!-- Issue: usedBy is not defined in ISO/IEC 5087-1. -->
    <!-- https://w3id.org/isoiec5087/-1/v1/usedBy -->

    <owl:ObjectProperty rdf:about="https://w3id.org/isoiec5087/-1/v1/usedBy">
        <rdfs:subPropertyOf rdf:resource="https://w3id.org/isoiec5087/-1/v1/preconditionOf"/>
        <rdfs:subPropertyOf rdf:resource="https://w3id.org/isoiec5087/-1/v1/ResourceObjectProperty"/>
    </owl:ObjectProperty>
    


    <!-- 
    ///////////////////////////////////////////////////////////////////////////////////////
    //
    // Classes
    //
    ///////////////////////////////////////////////////////////////////////////////////////
     -->

    
    <!-- https://w3id.org/isoiec5087/-1/v1/ConsumeState -->

    <owl:Class rdf:about="https://w3id.org/isoiec5087/-1/v1/ConsumeState">
        <skos:definition>Identifies a Resource and Quantity it consumes. The Quantity is removed from the Resource.</skos:definition>
        <rdfs:subClassOf rdf:resource="https://w3id.org/isoiec5087/-1/v1/TerminalResourceState"/>
    </owl:Class>
    


    <!-- https://w3id.org/isoiec5087/-1/v1/DivisibleResource -->

    <owl:Class rdf:about="https://w3id.org/isoiec5087/-1/v1/DivisibleResource">
        <skos:definition>A Resource that can be divided for use or consumption between multiple Activities.</skos:definition>
        <rdfs:subClassOf rdf:resource="https://w3id.org/isoiec5087/-1/v1/Resource"/>
    </owl:Class>
    


    <!-- https://w3id.org/isoiec5087/-1/v1/NonDivisibleResource -->

    <owl:Class rdf:about="https://w3id.org/isoiec5087/-1/v1/NonDivisibleResource">
        <skos:definition>A Resource that can only be used for a single Activity at once - even if it isn't fully utilized.</skos:definition>
        <rdfs:subClassOf rdf:resource="https://w3id.org/isoiec5087/-1/v1/Resource"/>
    </owl:Class>
    

    <!-- Issue: PlannedAllocation is not defined to be of type Manifestation in ISO/IEC 5087-1. -->
    <!-- https://w3id.org/isoiec5087/-1/v1/PlannedAllocation -->

    <owl:Class rdf:about="https://w3id.org/isoiec5087/-1/v1/PlannedAllocation">
        <skos:definition xml:lang="en">Specifies the planned allocation of a resource to an activity via a state.
        Note that Allocation is a Manifestation as the allocation may change over time.</skos:definition>
        <rdfs:subClassOf rdf:resource="https://w3id.org/isoiec5087/-1/v1/Manifestation"/>
        <rdfs:subClassOf rdf:resource="https://w3id.org/isoiec5087/-1/v1/ResourceThing"/>
        <rdfs:subClassOf>
            <owl:Restriction>
                <owl:onProperty rdf:resource="http://www.w3.org/2006/time#hasTime"/>
                <owl:qualifiedCardinality rdf:datatype="http://www.w3.org/2001/XMLSchema#nonNegativeInteger">1</owl:qualifiedCardinality>
                <owl:onClass rdf:resource="http://www.w3.org/2006/time#TemporalEntity"/>
            </owl:Restriction>
        </rdfs:subClassOf>
        <rdfs:subClassOf>
            <owl:Restriction>
                <owl:onProperty rdf:resource="https://w3id.org/isoiec5087/-1/v1/forResource"/>
                <owl:qualifiedCardinality rdf:datatype="http://www.w3.org/2001/XMLSchema#nonNegativeInteger">1</owl:qualifiedCardinality>
                <owl:onClass rdf:resource="https://w3id.org/isoiec5087/-1/v1/Resource"/>
            </owl:Restriction>
        </rdfs:subClassOf>
        <rdfs:subClassOf>
            <owl:Restriction>
                <owl:onProperty rdf:resource="https://w3id.org/isoiec5087/-1/v1/forState"/>
                <owl:qualifiedCardinality rdf:datatype="http://www.w3.org/2001/XMLSchema#nonNegativeInteger">1</owl:qualifiedCardinality>
                <owl:onClass rdf:resource="https://w3id.org/isoiec5087/-1/v1/State"/>
            </owl:Restriction>
        </rdfs:subClassOf>
        <rdfs:subClassOf>
            <owl:Restriction>
                <owl:onProperty rdf:resource="https://w3id.org/isoiec5087/-1/v1/hasQuantity"/>
                <owl:qualifiedCardinality rdf:datatype="http://www.w3.org/2001/XMLSchema#nonNegativeInteger">1</owl:qualifiedCardinality>
                <owl:onClass rdf:resource="https://w3id.org/isoiec21972/v1/Quantity"/>
            </owl:Restriction>
        </rdfs:subClassOf>
    </owl:Class>
    


    <!-- https://w3id.org/isoiec5087/-1/v1/ProduceState -->

    <owl:Class rdf:about="https://w3id.org/isoiec5087/-1/v1/ProduceState">
        <skos:definition>Identifies a Resource and Quantity it produces.</skos:definition>
        <rdfs:subClassOf rdf:resource="https://w3id.org/isoiec5087/-1/v1/TerminalResourceState"/>
    </owl:Class>
    


    <!-- https://w3id.org/isoiec5087/-1/v1/ReleaseState -->

    <owl:Class rdf:about="https://w3id.org/isoiec5087/-1/v1/ReleaseState">
        <skos:definition>Identifies a Resource and Quantity it releases (after using).</skos:definition>
        <rdfs:subClassOf rdf:resource="https://w3id.org/isoiec5087/-1/v1/TerminalResourceState"/>
    </owl:Class>
    


    <!-- https://w3id.org/isoiec5087/-1/v1/Resource -->

    <owl:Class rdf:about="https://w3id.org/isoiec5087/-1/v1/Resource">
        <skos:definition>A Resource is a generic representation of some Thing that can be &quot;used&quot; in an Activity. 
        A Resource may have some Location, amount or availability, according to the definition of the Manifestation or TimeVaryingEntity. 
        A Resource must be classified as some Resource Type.
        A Resource may participate in some Activity Occurrence. In other words, it links to the Activity that the Resource is being used/consumed/produced/released at the time of the manifestation.
        A specific Resource may be used in or consumed in some activity occurrence.</skos:definition>
        <rdfs:subClassOf rdf:resource="https://w3id.org/isoiec5087/-1/v1/ResourceThing"/>
        <rdfs:subClassOf>
            <owl:Restriction>
                <owl:onProperty rdf:resource="https://w3id.org/isoiec5087/-1/v1/hasLocation"/>
                <owl:allValuesFrom rdf:resource="https://w3id.org/isoiec5087/-1/v1/Location"/>
            </owl:Restriction>
        </rdfs:subClassOf>
        <rdfs:subClassOf>
            <owl:Restriction>
                <owl:onProperty rdf:resource="https://w3id.org/isoiec5087/-1/v1/hasAllocation"/>
                <owl:allValuesFrom rdf:resource="https://w3id.org/isoiec5087/-1/v1/PlannedAllocation"/>
            </owl:Restriction>
        </rdfs:subClassOf>
        <rdfs:subClassOf>
            <owl:Restriction>
                <owl:onProperty rdf:resource="https://w3id.org/isoiec5087/-1/v1/participatesIn"/>
                <!-- Issue: Resource.participatesIn is defined as only Activity in ISO/IEC 5087-1 rather than min 1 -->
                <owl:minQualifiedCardinality rdf:datatype="http://www.w3.org/2001/XMLSchema#nonNegativeInteger">1</owl:minQualifiedCardinality>
                <owl:onClass rdf:resource="https://w3id.org/isoiec5087/-1/v1/Activity"/>
            </owl:Restriction>
        </rdfs:subClassOf>
        <rdfs:subClassOf>
            <owl:Restriction>
                <owl:onProperty rdf:resource="https://w3id.org/isoiec5087/-1/v1/capacityInUse"/>
                <owl:qualifiedCardinality rdf:datatype="http://www.w3.org/2001/XMLSchema#nonNegativeInteger">1</owl:qualifiedCardinality>
                <owl:onClass rdf:resource="https://w3id.org/isoiec21972/v1/Quantity"/>
            </owl:Restriction>
        </rdfs:subClassOf>
        <rdfs:subClassOf>
            <owl:Restriction>
                <owl:onProperty rdf:resource="https://w3id.org/isoiec5087/-1/v1/hasAvailableCapacity"/>
                <owl:qualifiedCardinality rdf:datatype="http://www.w3.org/2001/XMLSchema#nonNegativeInteger">1</owl:qualifiedCardinality>
                <owl:onClass rdf:resource="https://w3id.org/isoiec21972/v1/Quantity"/>
            </owl:Restriction>
        </rdfs:subClassOf>
        <rdfs:subClassOf>
            <owl:Restriction>
                <owl:onProperty rdf:resource="https://w3id.org/isoiec5087/-1/v1/hasCapacity"/>
                <owl:qualifiedCardinality rdf:datatype="http://www.w3.org/2001/XMLSchema#nonNegativeInteger">1</owl:qualifiedCardinality>
                <owl:onClass rdf:resource="https://w3id.org/isoiec21972/v1/Quantity"/>
            </owl:Restriction>
        </rdfs:subClassOf>
        <owl:disjointUnionOf rdf:parseType="Collection">
            <rdf:Description rdf:about="https://w3id.org/isoiec5087/-1/v1/DivisibleResource"/>
            <rdf:Description rdf:about="https://w3id.org/isoiec5087/-1/v1/NonDivisibleResource"/>
        </owl:disjointUnionOf>
    </owl:Class>
    


    <!-- https://w3id.org/isoiec5087/-1/v1/ResourceThing -->

    <owl:Class rdf:about="https://w3id.org/isoiec5087/-1/v1/ResourceThing">
        <skos:definition>Added for organizational purposes, to identify all classes defined in the Resource ontology.</skos:definition>
        <rdfs:subClassOf rdf:resource="https://w3id.org/isoiec5087/-1/v1/FoundationalCdmThing"/>
    </owl:Class>
    

    <!-- Issue: No definition provided for ResourceState -->
    <!-- https://w3id.org/isoiec5087/-1/v1/TerminalResourceState -->

    <owl:Class rdf:about="https://w3id.org/isoiec5087/-1/v1/TerminalResourceState">
        <skos:definition></skos:definition>
        <rdfs:subClassOf rdf:resource="https://w3id.org/isoiec5087/-1/v1/TerminalState"/>
        <rdfs:subClassOf rdf:resource="https://w3id.org/isoiec5087/-1/v1/ResourceThing"/>
        <rdfs:subClassOf>
            <owl:Restriction>
                <owl:onProperty rdf:resource="https://w3id.org/isoiec5087/-1/v1/hasAllocation"/>
                <owl:allValuesFrom rdf:resource="https://w3id.org/isoiec5087/-1/v1/PlannedAllocation"/>
            </owl:Restriction>
        </rdfs:subClassOf>
        <rdfs:subClassOf>
            <owl:Restriction>
                <owl:onProperty rdf:resource="https://w3id.org/isoiec5087/-1/v1/hasQuantity"/>
                <owl:allValuesFrom rdf:resource="https://w3id.org/isoiec21972/v1/Quantity"/>
            </owl:Restriction>
        </rdfs:subClassOf>
        <rdfs:subClassOf>
            <owl:Restriction>
                <owl:onProperty rdf:resource="https://w3id.org/isoiec5087/-1/v1/hasResource"/>
                <owl:allValuesFrom rdf:resource="https://w3id.org/isoiec5087/-1/v1/Resource"/>
            </owl:Restriction>
        </rdfs:subClassOf>
    </owl:Class>
    


    <!-- https://w3id.org/isoiec5087/-1/v1/UseState -->

    <owl:Class rdf:about="https://w3id.org/isoiec5087/-1/v1/UseState">
        <skos:definition>Identifies a Resource and Quantity it uses (without consuming).</skos:definition>
        <rdfs:subClassOf rdf:resource="https://w3id.org/isoiec5087/-1/v1/TerminalResourceState"/>
    </owl:Class>

    


    <!-- 
    ///////////////////////////////////////////////////////////////////////////////////////
    //
    // Object Properties
    //
    ///////////////////////////////////////////////////////////////////////////////////////
     -->

    
    <!-- https://w3id.org/isoiec5087/-1/v1/hasLocation -->

    <owl:ObjectProperty rdf:about="https://w3id.org/isoiec5087/-1/v1/hasLocation">
        <skos:definition>Specifies the Location of an object.</skos:definition>
        <rdfs:subPropertyOf rdf:resource="https://w3id.org/isoiec5087/-1/v1/LocationObjectProperty"/>
        <rdfs:range rdf:resource="https://w3id.org/isoiec5087/-1/v1/Location"/>
    </owl:ObjectProperty>
    

    <!-- Issue: No definition provided for nonTangentialProperPart -->
    <!-- https://w3id.org/isoiec5087/-1/v1/nonTangentialProperPart -->

    <owl:ObjectProperty rdf:about="https://w3id.org/isoiec5087/-1/v1/nonTangentialProperPart">
        <rdfs:subPropertyOf rdf:resource="http://www.opengis.net/ont/geosparql#rcc8ntpp"/>
        <rdfs:subPropertyOf rdf:resource="https://w3id.org/isoiec5087/-1/v1/properPartOf"/>
    </owl:ObjectProperty>
    

    <!-- Issue: No definition provided for tangentialProperPart -->
    <!-- https://w3id.org/isoiec5087/-1/v1/tangentialProperPart -->

    <owl:ObjectProperty rdf:about="https://w3id.org/isoiec5087/-1/v1/tangentialProperPart">
        <rdfs:subPropertyOf rdf:resource="http://www.opengis.net/ont/geosparql#rcc8tpp"/>
        <rdfs:subPropertyOf rdf:resource="https://w3id.org/isoiec5087/-1/v1/properPartOf"/>
    </owl:ObjectProperty>
    
    <!-- Issue: as_nDLatLon is not defined in ISO/IEC 5087-1 -->
    <!-- https://w3id.org/isoiec5087/-1/v1/as_nDLatLon -->

    <owl:DatatypeProperty rdf:about="https://w3id.org/isoiec5087/-1/v1/as_nDLatLon">
        <rdfs:subPropertyOf rdf:resource="https://w3id.org/isoiec5087/-1/v1/hasSerialization"/>
        <rdfs:domain rdf:resource="http://www.opengis.net/ont/sf#Geometry"/>
        <rdfs:range rdf:resource="http://franz.com/ns/allegrograph/5.0/geo/nd#_lat_la_-9.+1_+9.+1_+1.-4_+1.-1_lon_lo_-1.8+2_+1.8+2_+1.-4"/>
    </owl:DatatypeProperty>
    

    <!-- Issue: hasSerialization is not defined in ISO/IEC 5087-1 -->
    <!-- https://w3id.org/isoiec5087/-1/v1/hasSerialization -->

    <owl:DatatypeProperty rdf:about="https://w3id.org/isoiec5087/-1/v1/hasSerialization">
        <rdfs:subPropertyOf rdf:resource="https://w3id.org/isoiec5087/-1/v1/SpatialLocDataProperty"/>
    </owl:DatatypeProperty>
    
</rdf:RDF>


    <!-- https://w3id.org/citydata/test/isInvariant -->

    <owl:AnnotationProperty rdf:about="https://w3id.org/citydata/test/isInvariant">
        <rdfs:comment xml:lang="en">Identifies whether a property is to be interpreted as invariant (i.e., its value is not subject to change over time).</rdfs:comment>
        <rdfs:range rdf:resource="http://www.w3.org/2001/XMLSchema#boolean"/>
    </owl:AnnotationProperty>
    
